rt refine: Lots of progress proving schedule_invs'.
* Tweaked the definition of valid_sched_context so that scRefillHead is
  strictly less than scRefillMax.
* There are remaining problems where we need to know that certain
  scheduling contexts are active.

Signed-off-by: Mitchell Buckley <mitchell.buckley@data61.csiro.au>

proof/refine/ARM/Invariants_H.thy
@@ -630,7 +630,7 @@ definition valid_sched_context' :: "sched_context \<Rightarrow> kernel_state \<R
      \<and> MIN_REFILLS \<le> length (scRefills sc)
      \<and> scRefillMax sc \<le> length (scRefills sc)
      \<and> (0 < scRefillMax sc \<longrightarrow>
-          scRefillHead sc \<le> scRefillMax sc \<and> scRefillCount sc \<le> scRefillMax sc)"
+          scRefillHead sc < scRefillMax sc \<and> scRefillCount sc \<le> scRefillMax sc)"
 
 definition valid_reply' :: "reply \<Rightarrow> kernel_state \<Rightarrow> bool" where
   "valid_reply' reply s \<equiv>
